auto_generated/isabelle/Memory_image_orderings.thy
@@ -66,133 +66,133 @@ begin
 (*open import Missing_pervasives*)
 
 (*val elfFileFeatureCompare : elf_file_feature -> elf_file_feature -> Basic_classes.ordering*)
-fun elfFileFeatureCompare0  :: " elf_file_feature \<Rightarrow> elf_file_feature \<Rightarrow> ordering "  where 
-     " elfFileFeatureCompare0 (ElfHeader0(x1)) (ElfHeader0(x2)) = ( (* equal tags, so ... *) elf64_header_compare x1 x2 )"
-|" elfFileFeatureCompare0 (ElfHeader0(x1)) _ = ( LT )"
-|" elfFileFeatureCompare0 (ElfSectionHeaderTable0(x1)) (ElfHeader0(x2)) = ( GT )"
-|" elfFileFeatureCompare0 (ElfSectionHeaderTable0(x1)) (ElfSectionHeaderTable0(x2)) = ( ( (* equal tags, so ... *)lexicographicCompareBy compare_elf64_section_header_table_entry x1 x2))"
-|" elfFileFeatureCompare0 (ElfSectionHeaderTable0(x1)) _ = ( LT )"
-|" elfFileFeatureCompare0 (ElfProgramHeaderTable0(x1)) (ElfHeader0(x2)) = ( GT )"
-|" elfFileFeatureCompare0 (ElfProgramHeaderTable0(x1)) (ElfSectionHeaderTable0(x2)) = ( GT )"
-|" elfFileFeatureCompare0 (ElfProgramHeaderTable0(x1)) (ElfProgramHeaderTable0(x2)) = ( (lexicographicCompareBy compare_elf64_program_header_table_entry x1 x2))"
-|" elfFileFeatureCompare0 (ElfProgramHeaderTable0(x1)) _ = ( LT )"
-|" elfFileFeatureCompare0 (ElfSection0(x1)) (ElfHeader0(x2)) = ( GT )"
-|" elfFileFeatureCompare0 (ElfSection0(x1)) (ElfSectionHeaderTable0(x2)) = ( GT )"
-|" elfFileFeatureCompare0 (ElfSection0(x1)) (ElfProgramHeaderTable0(x2)) = ( GT )"
-|" elfFileFeatureCompare0 (ElfSection0(x1)) (ElfSection0(x2)) = ( (pairCompare (genericCompare (op<) (op=)) compare_elf64_interpreted_section x1 x2))"
-|" elfFileFeatureCompare0 (ElfSection0(x1)) _ = ( LT )"
-|" elfFileFeatureCompare0 (ElfSegment0(x1)) (ElfHeader0(x2)) = ( GT )"
-|" elfFileFeatureCompare0 (ElfSegment0(x1)) (ElfSectionHeaderTable0(x2)) = ( GT )"
-|" elfFileFeatureCompare0 (ElfSegment0(x1)) (ElfProgramHeaderTable0(x2)) = ( GT )"
-|" elfFileFeatureCompare0 (ElfSegment0(x1)) (ElfSection0(x2)) = ( GT )"
-|" elfFileFeatureCompare0 (ElfSegment0(x1)) (ElfSegment0(x2)) = ( (pairCompare (genericCompare (op<) (op=)) compare_elf64_interpreted_segment x1 x2))" 
-declare elfFileFeatureCompare0.simps [simp del]
+fun elfFileFeatureCompare  :: " elf_file_feature \<Rightarrow> elf_file_feature \<Rightarrow> ordering "  where 
+     " elfFileFeatureCompare (ElfHeader(x1)) (ElfHeader(x2)) = ( (* equal tags, so ... *) elf64_header_compare x1 x2 )"
+|" elfFileFeatureCompare (ElfHeader(x1)) _ = ( LT )"
+|" elfFileFeatureCompare (ElfSectionHeaderTable(x1)) (ElfHeader(x2)) = ( GT )"
+|" elfFileFeatureCompare (ElfSectionHeaderTable(x1)) (ElfSectionHeaderTable(x2)) = ( ( (* equal tags, so ... *)lexicographicCompareBy compare_elf64_section_header_table_entry x1 x2))"
+|" elfFileFeatureCompare (ElfSectionHeaderTable(x1)) _ = ( LT )"
+|" elfFileFeatureCompare (ElfProgramHeaderTable(x1)) (ElfHeader(x2)) = ( GT )"
+|" elfFileFeatureCompare (ElfProgramHeaderTable(x1)) (ElfSectionHeaderTable(x2)) = ( GT )"
+|" elfFileFeatureCompare (ElfProgramHeaderTable(x1)) (ElfProgramHeaderTable(x2)) = ( (lexicographicCompareBy compare_elf64_program_header_table_entry x1 x2))"
+|" elfFileFeatureCompare (ElfProgramHeaderTable(x1)) _ = ( LT )"
+|" elfFileFeatureCompare (ElfSection(x1)) (ElfHeader(x2)) = ( GT )"
+|" elfFileFeatureCompare (ElfSection(x1)) (ElfSectionHeaderTable(x2)) = ( GT )"
+|" elfFileFeatureCompare (ElfSection(x1)) (ElfProgramHeaderTable(x2)) = ( GT )"
+|" elfFileFeatureCompare (ElfSection(x1)) (ElfSection(x2)) = ( (pairCompare (genericCompare (op<) (op=)) compare_elf64_interpreted_section x1 x2))"
+|" elfFileFeatureCompare (ElfSection(x1)) _ = ( LT )"
+|" elfFileFeatureCompare (ElfSegment(x1)) (ElfHeader(x2)) = ( GT )"
+|" elfFileFeatureCompare (ElfSegment(x1)) (ElfSectionHeaderTable(x2)) = ( GT )"
+|" elfFileFeatureCompare (ElfSegment(x1)) (ElfProgramHeaderTable(x2)) = ( GT )"
+|" elfFileFeatureCompare (ElfSegment(x1)) (ElfSection(x2)) = ( GT )"
+|" elfFileFeatureCompare (ElfSegment(x1)) (ElfSegment(x2)) = ( (pairCompare (genericCompare (op<) (op=)) compare_elf64_interpreted_segment x1 x2))" 
+declare elfFileFeatureCompare.simps [simp del]
 
 
 (*val elfFileFeatureTagEquiv : elf_file_feature -> elf_file_feature -> bool*)
-fun elfFileFeatureTagEquiv0  :: " elf_file_feature \<Rightarrow> elf_file_feature \<Rightarrow> bool "  where 
-     " elfFileFeatureTagEquiv0 (ElfHeader0(x1)) (ElfHeader0(x2)) = ( (* equal tags, so ... *) True )"
-|" elfFileFeatureTagEquiv0 (ElfSectionHeaderTable0(x1)) (ElfSectionHeaderTable0(x2)) = ( True )"
-|" elfFileFeatureTagEquiv0 (ElfProgramHeaderTable0(x1)) (ElfProgramHeaderTable0(x2)) = ( True )"
-|" elfFileFeatureTagEquiv0 (ElfSection0(x1)) (ElfSection0(x2)) = ( True )"
-|" elfFileFeatureTagEquiv0 (ElfSegment0(x1)) (ElfSegment0(x2)) = ( True )"
-|" elfFileFeatureTagEquiv0 _ _ = ( False )" 
-declare elfFileFeatureTagEquiv0.simps [simp del]
+fun elfFileFeatureTagEquiv  :: " elf_file_feature \<Rightarrow> elf_file_feature \<Rightarrow> bool "  where 
+     " elfFileFeatureTagEquiv (ElfHeader(x1)) (ElfHeader(x2)) = ( (* equal tags, so ... *) True )"
+|" elfFileFeatureTagEquiv (ElfSectionHeaderTable(x1)) (ElfSectionHeaderTable(x2)) = ( True )"
+|" elfFileFeatureTagEquiv (ElfProgramHeaderTable(x1)) (ElfProgramHeaderTable(x2)) = ( True )"
+|" elfFileFeatureTagEquiv (ElfSection(x1)) (ElfSection(x2)) = ( True )"
+|" elfFileFeatureTagEquiv (ElfSegment(x1)) (ElfSegment(x2)) = ( True )"
+|" elfFileFeatureTagEquiv _ _ = ( False )" 
+declare elfFileFeatureTagEquiv.simps [simp del]
 
 
-definition instance_Basic_classes_Ord_Memory_image_elf_file_feature_dict0  :: "(elf_file_feature)Ord_class "  where 
-     " instance_Basic_classes_Ord_Memory_image_elf_file_feature_dict0 = ((|
+definition instance_Basic_classes_Ord_Memory_image_elf_file_feature_dict  :: "(elf_file_feature)Ord_class "  where 
+     " instance_Basic_classes_Ord_Memory_image_elf_file_feature_dict = ((|
 
-  compare_method = elfFileFeatureCompare0,
+  compare_method = elfFileFeatureCompare,
 
-  isLess_method = (\<lambda> f1 .  (\<lambda> f2 .  (elfFileFeatureCompare0 f1 f2 = LT))),
+  isLess_method = (\<lambda> f1 .  (\<lambda> f2 .  (elfFileFeatureCompare f1 f2 = LT))),
 
-  isLessEqual_method = (\<lambda> f1 .  (\<lambda> f2 .  (op \<in>) (elfFileFeatureCompare0 f1 f2) ({LT, EQ}))),
+  isLessEqual_method = (\<lambda> f1 .  (\<lambda> f2 .  (op \<in>) (elfFileFeatureCompare f1 f2) ({LT, EQ}))),
 
-  isGreater_method = (\<lambda> f1 .  (\<lambda> f2 .  (elfFileFeatureCompare0 f1 f2 = GT))),
+  isGreater_method = (\<lambda> f1 .  (\<lambda> f2 .  (elfFileFeatureCompare f1 f2 = GT))),
 
-  isGreaterEqual_method = (\<lambda> f1 .  (\<lambda> f2 .  (op \<in>) (elfFileFeatureCompare0 f1 f2) ({GT, EQ})))|) )"
+  isGreaterEqual_method = (\<lambda> f1 .  (\<lambda> f2 .  (op \<in>) (elfFileFeatureCompare f1 f2) ({GT, EQ})))|) )"
 
 
 (*val tagCompare : forall 'abifeature. Ord 'abifeature =>
     range_tag 'abifeature -> range_tag 'abifeature -> Basic_classes.ordering*)
-fun tagCompare0  :: " 'abifeature Ord_class \<Rightarrow> 'abifeature range_tag \<Rightarrow> 'abifeature range_tag \<Rightarrow> ordering "  where 
-     " tagCompare0 dict_Basic_classes_Ord_abifeature ImageBase0 ImageBase0 = ( EQ )"
-|" tagCompare0 dict_Basic_classes_Ord_abifeature ImageBase0 _ = ( LT )"
-|" tagCompare0 dict_Basic_classes_Ord_abifeature EntryPoint0 ImageBase0 = ( GT )"
-|" tagCompare0 dict_Basic_classes_Ord_abifeature EntryPoint0 EntryPoint0 = ( EQ )"
-|" tagCompare0 dict_Basic_classes_Ord_abifeature EntryPoint0 _ = ( LT )"
-|" tagCompare0 dict_Basic_classes_Ord_abifeature (SymbolDef0(_)) ImageBase0 = ( GT )"
-|" tagCompare0 dict_Basic_classes_Ord_abifeature (SymbolDef0(_)) EntryPoint0 = ( GT )"
-|" tagCompare0 dict_Basic_classes_Ord_abifeature (SymbolDef0(x1)) (SymbolDef0(x2)) = ( symDefCompare0 x1 x2 )"
-|" tagCompare0 dict_Basic_classes_Ord_abifeature (SymbolDef0(_)) _ = ( LT )"
-|" tagCompare0 dict_Basic_classes_Ord_abifeature (SymbolRef0(_)) ImageBase0 = ( GT )"
-|" tagCompare0 dict_Basic_classes_Ord_abifeature (SymbolRef0(_)) EntryPoint0 = ( GT )"
-|" tagCompare0 dict_Basic_classes_Ord_abifeature (SymbolRef0(_)) (SymbolDef0(_)) = ( GT )"
-|" tagCompare0 dict_Basic_classes_Ord_abifeature (SymbolRef0(x1)) (SymbolRef0(x2)) = ( symRefAndRelocSiteCompare0 x1 x2 )"
-|" tagCompare0 dict_Basic_classes_Ord_abifeature (SymbolRef0(_)) _ = ( LT )"
-|" tagCompare0 dict_Basic_classes_Ord_abifeature (FileFeature0(_)) ImageBase0 = ( GT )"
-|" tagCompare0 dict_Basic_classes_Ord_abifeature (FileFeature0(_)) EntryPoint0 = ( GT )"
-|" tagCompare0 dict_Basic_classes_Ord_abifeature (FileFeature0(_)) (SymbolDef0(_)) = ( GT )"
-|" tagCompare0 dict_Basic_classes_Ord_abifeature (FileFeature0(_)) (SymbolRef0(_)) = ( GT )"
-|" tagCompare0 dict_Basic_classes_Ord_abifeature (FileFeature0(x1)) (FileFeature0(x2)) = ( elfFileFeatureCompare0 x1 x2 )"
-|" tagCompare0 dict_Basic_classes_Ord_abifeature (FileFeature0(_)) _ = ( LT )"
-|" tagCompare0 dict_Basic_classes_Ord_abifeature (AbiFeature0(_)) ImageBase0 = ( GT )"
-|" tagCompare0 dict_Basic_classes_Ord_abifeature (AbiFeature0(_)) EntryPoint0 = ( GT )"
-|" tagCompare0 dict_Basic_classes_Ord_abifeature (AbiFeature0(_)) (SymbolDef0(_)) = ( GT )"
-|" tagCompare0 dict_Basic_classes_Ord_abifeature (AbiFeature0(_)) (SymbolRef0(_)) = ( GT )"
-|" tagCompare0 dict_Basic_classes_Ord_abifeature (AbiFeature0(_)) (FileFeature0(_)) = ( GT )"
-|" tagCompare0 dict_Basic_classes_Ord_abifeature (AbiFeature0(x1)) (AbiFeature0(x2)) = (
+fun tagCompare  :: " 'abifeature Ord_class \<Rightarrow> 'abifeature range_tag \<Rightarrow> 'abifeature range_tag \<Rightarrow> ordering "  where 
+     " tagCompare dict_Basic_classes_Ord_abifeature ImageBase ImageBase = ( EQ )"
+|" tagCompare dict_Basic_classes_Ord_abifeature ImageBase _ = ( LT )"
+|" tagCompare dict_Basic_classes_Ord_abifeature EntryPoint ImageBase = ( GT )"
+|" tagCompare dict_Basic_classes_Ord_abifeature EntryPoint EntryPoint = ( EQ )"
+|" tagCompare dict_Basic_classes_Ord_abifeature EntryPoint _ = ( LT )"
+|" tagCompare dict_Basic_classes_Ord_abifeature (SymbolDef(_)) ImageBase = ( GT )"
+|" tagCompare dict_Basic_classes_Ord_abifeature (SymbolDef(_)) EntryPoint = ( GT )"
+|" tagCompare dict_Basic_classes_Ord_abifeature (SymbolDef(x1)) (SymbolDef(x2)) = ( symDefCompare x1 x2 )"
+|" tagCompare dict_Basic_classes_Ord_abifeature (SymbolDef(_)) _ = ( LT )"
+|" tagCompare dict_Basic_classes_Ord_abifeature (SymbolRef(_)) ImageBase = ( GT )"
+|" tagCompare dict_Basic_classes_Ord_abifeature (SymbolRef(_)) EntryPoint = ( GT )"
+|" tagCompare dict_Basic_classes_Ord_abifeature (SymbolRef(_)) (SymbolDef(_)) = ( GT )"
+|" tagCompare dict_Basic_classes_Ord_abifeature (SymbolRef(x1)) (SymbolRef(x2)) = ( symRefAndRelocSiteCompare x1 x2 )"
+|" tagCompare dict_Basic_classes_Ord_abifeature (SymbolRef(_)) _ = ( LT )"
+|" tagCompare dict_Basic_classes_Ord_abifeature (FileFeature(_)) ImageBase = ( GT )"
+|" tagCompare dict_Basic_classes_Ord_abifeature (FileFeature(_)) EntryPoint = ( GT )"
+|" tagCompare dict_Basic_classes_Ord_abifeature (FileFeature(_)) (SymbolDef(_)) = ( GT )"
+|" tagCompare dict_Basic_classes_Ord_abifeature (FileFeature(_)) (SymbolRef(_)) = ( GT )"
+|" tagCompare dict_Basic_classes_Ord_abifeature (FileFeature(x1)) (FileFeature(x2)) = ( elfFileFeatureCompare x1 x2 )"
+|" tagCompare dict_Basic_classes_Ord_abifeature (FileFeature(_)) _ = ( LT )"
+|" tagCompare dict_Basic_classes_Ord_abifeature (AbiFeature(_)) ImageBase = ( GT )"
+|" tagCompare dict_Basic_classes_Ord_abifeature (AbiFeature(_)) EntryPoint = ( GT )"
+|" tagCompare dict_Basic_classes_Ord_abifeature (AbiFeature(_)) (SymbolDef(_)) = ( GT )"
+|" tagCompare dict_Basic_classes_Ord_abifeature (AbiFeature(_)) (SymbolRef(_)) = ( GT )"
+|" tagCompare dict_Basic_classes_Ord_abifeature (AbiFeature(_)) (FileFeature(_)) = ( GT )"
+|" tagCompare dict_Basic_classes_Ord_abifeature (AbiFeature(x1)) (AbiFeature(x2)) = (
   (compare_method   dict_Basic_classes_Ord_abifeature) x1 x2 )" 
-declare tagCompare0.simps [simp del]
+declare tagCompare.simps [simp del]
 
 
-definition instance_Basic_classes_Ord_Memory_image_range_tag_dict1  :: " 'abifeature Ord_class \<Rightarrow>('abifeature range_tag)Ord_class "  where 
-     " instance_Basic_classes_Ord_Memory_image_range_tag_dict1 dict_Basic_classes_Ord_abifeature = ((|
+definition instance_Basic_classes_Ord_Memory_image_range_tag_dict  :: " 'abifeature Ord_class \<Rightarrow>('abifeature range_tag)Ord_class "  where 
+     " instance_Basic_classes_Ord_Memory_image_range_tag_dict dict_Basic_classes_Ord_abifeature = ((|
 
   compare_method = 
-  (tagCompare0 dict_Basic_classes_Ord_abifeature),
+  (tagCompare dict_Basic_classes_Ord_abifeature),
 
-  isLess_method = (\<lambda> tag1 .  (\<lambda> tag2 .  (tagCompare0 
+  isLess_method = (\<lambda> tag1 .  (\<lambda> tag2 .  (tagCompare 
   dict_Basic_classes_Ord_abifeature tag1 tag2 = LT))),
 
-  isLessEqual_method = (\<lambda> tag1 .  (\<lambda> tag2 .  (op \<in>) (tagCompare0 
+  isLessEqual_method = (\<lambda> tag1 .  (\<lambda> tag2 .  (op \<in>) (tagCompare 
   dict_Basic_classes_Ord_abifeature tag1 tag2) ({LT, EQ}))),
 
-  isGreater_method = (\<lambda> tag1 .  (\<lambda> tag2 .  (tagCompare0 
+  isGreater_method = (\<lambda> tag1 .  (\<lambda> tag2 .  (tagCompare 
   dict_Basic_classes_Ord_abifeature tag1 tag2 = GT))),
 
-  isGreaterEqual_method = (\<lambda> tag1 .  (\<lambda> tag2 .  (op \<in>) (tagCompare0 
+  isGreaterEqual_method = (\<lambda> tag1 .  (\<lambda> tag2 .  (op \<in>) (tagCompare 
   dict_Basic_classes_Ord_abifeature tag1 tag2) ({GT, EQ})))|) )"
 
 
 (*val tagEquiv : forall 'abifeature. AbiFeatureTagEquiv 'abifeature => range_tag 'abifeature -> range_tag 'abifeature -> bool*)
-fun tagEquiv0  :: " 'abifeature AbiFeatureTagEquiv_class \<Rightarrow> 'abifeature range_tag \<Rightarrow> 'abifeature range_tag \<Rightarrow> bool "  where 
-     " tagEquiv0 dict_Abi_classes_AbiFeatureTagEquiv_abifeature ImageBase0 ImageBase0 = ( True )"
-|" tagEquiv0 dict_Abi_classes_AbiFeatureTagEquiv_abifeature EntryPoint0 EntryPoint0 = ( True )"
-|" tagEquiv0 dict_Abi_classes_AbiFeatureTagEquiv_abifeature (SymbolDef0(x1)) (SymbolDef0(x2)) = ( True )"
-|" tagEquiv0 dict_Abi_classes_AbiFeatureTagEquiv_abifeature (SymbolRef0(_)) (SymbolRef0(_)) = ( True )"
-|" tagEquiv0 dict_Abi_classes_AbiFeatureTagEquiv_abifeature (FileFeature0(x1)) (FileFeature0(x2)) = ( elfFileFeatureTagEquiv0 x1 x2 )"
-|" tagEquiv0 dict_Abi_classes_AbiFeatureTagEquiv_abifeature (AbiFeature0(x1)) (AbiFeature0(x2)) = (
+fun tagEquiv  :: " 'abifeature AbiFeatureTagEquiv_class \<Rightarrow> 'abifeature range_tag \<Rightarrow> 'abifeature range_tag \<Rightarrow> bool "  where 
+     " tagEquiv dict_Abi_classes_AbiFeatureTagEquiv_abifeature ImageBase ImageBase = ( True )"
+|" tagEquiv dict_Abi_classes_AbiFeatureTagEquiv_abifeature EntryPoint EntryPoint = ( True )"
+|" tagEquiv dict_Abi_classes_AbiFeatureTagEquiv_abifeature (SymbolDef(x1)) (SymbolDef(x2)) = ( True )"
+|" tagEquiv dict_Abi_classes_AbiFeatureTagEquiv_abifeature (SymbolRef(_)) (SymbolRef(_)) = ( True )"
+|" tagEquiv dict_Abi_classes_AbiFeatureTagEquiv_abifeature (FileFeature(x1)) (FileFeature(x2)) = ( elfFileFeatureTagEquiv x1 x2 )"
+|" tagEquiv dict_Abi_classes_AbiFeatureTagEquiv_abifeature (AbiFeature(x1)) (AbiFeature(x2)) = (
   (abiFeatureTagEquiv_method   dict_Abi_classes_AbiFeatureTagEquiv_abifeature) x1 x2 )"
-|" tagEquiv0 dict_Abi_classes_AbiFeatureTagEquiv_abifeature _ _ = ( False )" 
-declare tagEquiv0.simps [simp del]
+|" tagEquiv dict_Abi_classes_AbiFeatureTagEquiv_abifeature _ _ = ( False )" 
+declare tagEquiv.simps [simp del]
 
 
 (* ------- end of Ord / compare / ConstructorToNaturalList functions *)
 
 
 (*val unique_tag_matching : forall 'abifeature. Ord 'abifeature, AbiFeatureTagEquiv 'abifeature => range_tag 'abifeature -> annotated_memory_image 'abifeature -> range_tag 'abifeature*)
-definition unique_tag_matching0  :: " 'abifeature Ord_class \<Rightarrow> 'abifeature AbiFeatureTagEquiv_class \<Rightarrow> 'abifeature range_tag \<Rightarrow> 'abifeature annotated_memory_image \<Rightarrow> 'abifeature range_tag "  where 
-     " unique_tag_matching0 dict_Basic_classes_Ord_abifeature dict_Abi_classes_AbiFeatureTagEquiv_abifeature tag img2 = ( 
+definition unique_tag_matching  :: " 'abifeature Ord_class \<Rightarrow> 'abifeature AbiFeatureTagEquiv_class \<Rightarrow> 'abifeature range_tag \<Rightarrow> 'abifeature annotated_memory_image \<Rightarrow> 'abifeature range_tag "  where 
+     " unique_tag_matching dict_Basic_classes_Ord_abifeature dict_Abi_classes_AbiFeatureTagEquiv_abifeature tag img3 = ( 
     (case  Multimap.lookupBy0 
-  (instance_Basic_classes_Ord_Memory_image_range_tag_dict1
+  (instance_Basic_classes_Ord_Memory_image_range_tag_dict
      dict_Basic_classes_Ord_abifeature) (instance_Basic_classes_Ord_Maybe_maybe_dict
    (instance_Basic_classes_Ord_tup2_dict
       Lem_string_extra.instance_Basic_classes_Ord_string_dict
       (instance_Basic_classes_Ord_tup2_dict
          instance_Basic_classes_Ord_Num_natural_dict
-         instance_Basic_classes_Ord_Num_natural_dict)))  (tagEquiv0 dict_Abi_classes_AbiFeatureTagEquiv_abifeature) tag(by_tag0   img2) of
+         instance_Basic_classes_Ord_Num_natural_dict)))  (tagEquiv dict_Abi_classes_AbiFeatureTagEquiv_abifeature) tag(by_tag   img3) of
         [] => failwith (''no tag match found'')
         | [(t, r)] => t
         | x => failwith ((''more than one tag match'')) (* (ranges:  ^ 
@@ -202,21 +202,21 @@ definition unique_tag_matching0  :: " 'abifeature Ord_class \<Rightarrow> 'abife
 
     
 (*val tagged_ranges_matching_tag : forall 'abifeature. Ord 'abifeature, AbiFeatureTagEquiv 'abifeature => range_tag 'abifeature -> annotated_memory_image 'abifeature -> list (range_tag 'abifeature * maybe element_range)*)
-definition tagged_ranges_matching_tag0  :: " 'abifeature Ord_class \<Rightarrow> 'abifeature AbiFeatureTagEquiv_class \<Rightarrow> 'abifeature range_tag \<Rightarrow> 'abifeature annotated_memory_image \<Rightarrow>('abifeature range_tag*(element_range)option)list "  where 
-     " tagged_ranges_matching_tag0 dict_Basic_classes_Ord_abifeature dict_Abi_classes_AbiFeatureTagEquiv_abifeature tag img2 = ( 
+definition tagged_ranges_matching_tag  :: " 'abifeature Ord_class \<Rightarrow> 'abifeature AbiFeatureTagEquiv_class \<Rightarrow> 'abifeature range_tag \<Rightarrow> 'abifeature annotated_memory_image \<Rightarrow>('abifeature range_tag*(element_range)option)list "  where 
+     " tagged_ranges_matching_tag dict_Basic_classes_Ord_abifeature dict_Abi_classes_AbiFeatureTagEquiv_abifeature tag img3 = ( 
     Multimap.lookupBy0 
-  (instance_Basic_classes_Ord_Memory_image_range_tag_dict1
+  (instance_Basic_classes_Ord_Memory_image_range_tag_dict
      dict_Basic_classes_Ord_abifeature) (instance_Basic_classes_Ord_Maybe_maybe_dict
    (instance_Basic_classes_Ord_tup2_dict
       Lem_string_extra.instance_Basic_classes_Ord_string_dict
       (instance_Basic_classes_Ord_tup2_dict
          instance_Basic_classes_Ord_Num_natural_dict
-         instance_Basic_classes_Ord_Num_natural_dict)))  (tagEquiv0 dict_Abi_classes_AbiFeatureTagEquiv_abifeature) tag(by_tag0   img2))"
+         instance_Basic_classes_Ord_Num_natural_dict)))  (tagEquiv dict_Abi_classes_AbiFeatureTagEquiv_abifeature) tag(by_tag   img3))"
 
 
 (*val element_range_compare : element_range -> element_range -> Basic_classes.ordering*)
-definition element_range_compare0  :: " string*(nat*nat) \<Rightarrow> string*(nat*nat) \<Rightarrow> ordering "  where 
-     " element_range_compare0 = ( pairCompare (\<lambda> x y. EQ) (pairCompare (genericCompare (op<) (op=)) (genericCompare (op<) (op=))))"
+definition element_range_compare  :: " string*(nat*nat) \<Rightarrow> string*(nat*nat) \<Rightarrow> ordering "  where 
+     " element_range_compare = ( pairCompare (\<lambda> x y. EQ) (pairCompare (genericCompare (op<) (op=)) (genericCompare (op<) (op=))))"
 
 
 (*val unique_tag_matching_at_range_exact : forall 'abifeature. Ord 'abifeature, AbiFeatureTagEquiv 'abifeature =>
@@ -224,8 +224,8 @@ definition element_range_compare0  :: " string*(nat*nat) \<Rightarrow> string*(n
     -> range_tag 'abifeature
     -> annotated_memory_image 'abifeature
     -> range_tag 'abifeature*)
-definition unique_tag_matching_at_range_exact0  :: " 'abifeature Ord_class \<Rightarrow> 'abifeature AbiFeatureTagEquiv_class \<Rightarrow>(element_range)option \<Rightarrow> 'abifeature range_tag \<Rightarrow> 'abifeature annotated_memory_image \<Rightarrow> 'abifeature range_tag "  where 
-     " unique_tag_matching_at_range_exact0 dict_Basic_classes_Ord_abifeature dict_Abi_classes_AbiFeatureTagEquiv_abifeature r tag img2 = ( 
+definition unique_tag_matching_at_range_exact  :: " 'abifeature Ord_class \<Rightarrow> 'abifeature AbiFeatureTagEquiv_class \<Rightarrow>(element_range)option \<Rightarrow> 'abifeature range_tag \<Rightarrow> 'abifeature annotated_memory_image \<Rightarrow> 'abifeature range_tag "  where 
+     " unique_tag_matching_at_range_exact dict_Basic_classes_Ord_abifeature dict_Abi_classes_AbiFeatureTagEquiv_abifeature r tag img3 = ( 
     (* 1. find tags a unique range labelled as ELF section header table. *)
     (let (_, (allRangeMatches :: ( 'abifeature range_tag) list)) = (list_unzip (Multimap.lookupBy0 
   (instance_Basic_classes_Ord_Maybe_maybe_dict
@@ -233,10 +233,10 @@ definition unique_tag_matching_at_range_exact0  :: " 'abifeature Ord_class \<Rig
         Lem_string_extra.instance_Basic_classes_Ord_string_dict
         (instance_Basic_classes_Ord_tup2_dict
            instance_Basic_classes_Ord_Num_natural_dict
-           instance_Basic_classes_Ord_Num_natural_dict))) (instance_Basic_classes_Ord_Memory_image_range_tag_dict1
-   dict_Basic_classes_Ord_abifeature) (op=) r(by_range0   img2)))
+           instance_Basic_classes_Ord_Num_natural_dict))) (instance_Basic_classes_Ord_Memory_image_range_tag_dict
+   dict_Basic_classes_Ord_abifeature) (op=) r(by_range   img3)))
     in
-    (let (tagAlsoMatches :: ( 'abifeature range_tag) list) = (List.filter (\<lambda> x .  tagEquiv0 
+    (let (tagAlsoMatches :: ( 'abifeature range_tag) list) = (List.filter (\<lambda> x .  tagEquiv 
   dict_Abi_classes_AbiFeatureTagEquiv_abifeature x tag) allRangeMatches)
     in
     (case  tagAlsoMatches of
@@ -247,12 +247,12 @@ definition unique_tag_matching_at_range_exact0  :: " 'abifeature Ord_class \<Rig
 
 
 (*val symbol_def_ranges : forall 'abifeature. Ord 'abifeature, AbiFeatureTagEquiv 'abifeature => annotated_memory_image 'abifeature -> (list (range_tag 'abifeature) * list (maybe element_range))*)
-definition symbol_def_ranges0  :: " 'abifeature Ord_class \<Rightarrow> 'abifeature AbiFeatureTagEquiv_class \<Rightarrow> 'abifeature annotated_memory_image \<Rightarrow>('abifeature range_tag)list*((element_range)option)list "  where 
-     " symbol_def_ranges0 dict_Basic_classes_Ord_abifeature dict_Abi_classes_AbiFeatureTagEquiv_abifeature img2 = ( 
+definition symbol_def_ranges  :: " 'abifeature Ord_class \<Rightarrow> 'abifeature AbiFeatureTagEquiv_class \<Rightarrow> 'abifeature annotated_memory_image \<Rightarrow>('abifeature range_tag)list*((element_range)option)list "  where 
+     " symbol_def_ranges dict_Basic_classes_Ord_abifeature dict_Abi_classes_AbiFeatureTagEquiv_abifeature img3 = ( 
     (* find all element ranges labelled as ELF symbols *)
     (let (tags, maybe_ranges) = (list_unzip (
-        tagged_ranges_matching_tag0 
-  dict_Basic_classes_Ord_abifeature dict_Abi_classes_AbiFeatureTagEquiv_abifeature (SymbolDef0(null_symbol_definition0)) img2
+        tagged_ranges_matching_tag 
+  dict_Basic_classes_Ord_abifeature dict_Abi_classes_AbiFeatureTagEquiv_abifeature (SymbolDef(null_symbol_definition)) img3
     ))
     in
     (* some symbols, specifically ABS symbols, needn't label a range. *)
@@ -260,29 +260,29 @@ definition symbol_def_ranges0  :: " 'abifeature Ord_class \<Rightarrow> 'abifeat
 
 
 (*val name_of_symbol_def : symbol_definition -> string*)
-definition name_of_symbol_def0  :: " symbol_definition \<Rightarrow> string "  where 
-     " name_of_symbol_def0 sym1 = ((def_symname0   sym1))"
+definition name_of_symbol_def  :: " symbol_definition \<Rightarrow> string "  where 
+     " name_of_symbol_def sym1 = ((def_symname   sym1))"
 
 
 (*val defined_symbols_and_ranges : forall 'abifeature. Ord 'abifeature, AbiFeatureTagEquiv 'abifeature => annotated_memory_image 'abifeature -> list ((maybe element_range) * symbol_definition)*)
-definition defined_symbols_and_ranges0  :: " 'abifeature Ord_class \<Rightarrow> 'abifeature AbiFeatureTagEquiv_class \<Rightarrow> 'abifeature annotated_memory_image \<Rightarrow>((element_range)option*symbol_definition)list "  where 
-     " defined_symbols_and_ranges0 dict_Basic_classes_Ord_abifeature dict_Abi_classes_AbiFeatureTagEquiv_abifeature img2 = ( 
+definition defined_symbols_and_ranges  :: " 'abifeature Ord_class \<Rightarrow> 'abifeature AbiFeatureTagEquiv_class \<Rightarrow> 'abifeature annotated_memory_image \<Rightarrow>((element_range)option*symbol_definition)list "  where 
+     " defined_symbols_and_ranges dict_Basic_classes_Ord_abifeature dict_Abi_classes_AbiFeatureTagEquiv_abifeature img3 = ( 
     Lem_list.mapMaybe (\<lambda> (tag, maybeRange) .  
         (case  tag of
-            SymbolDef0(ent) => Some (maybeRange, ent)
+            SymbolDef(ent) => Some (maybeRange, ent)
             | _ => failwith (''impossible: non-symbol def in list of symbol defs'')
-        )) (tagged_ranges_matching_tag0 
-  dict_Basic_classes_Ord_abifeature dict_Abi_classes_AbiFeatureTagEquiv_abifeature (SymbolDef0(null_symbol_definition0)) img2))"
+        )) (tagged_ranges_matching_tag 
+  dict_Basic_classes_Ord_abifeature dict_Abi_classes_AbiFeatureTagEquiv_abifeature (SymbolDef(null_symbol_definition)) img3))"
 
 
 (*val defined_symbols : forall 'abifeature. Ord 'abifeature, AbiFeatureTagEquiv 'abifeature =>  annotated_memory_image 'abifeature -> list symbol_definition*)
-definition defined_symbols0  :: " 'abifeature Ord_class \<Rightarrow> 'abifeature AbiFeatureTagEquiv_class \<Rightarrow> 'abifeature annotated_memory_image \<Rightarrow>(symbol_definition)list "  where 
-     " defined_symbols0 dict_Basic_classes_Ord_abifeature dict_Abi_classes_AbiFeatureTagEquiv_abifeature img2 = ( 
-    (let (all_symbol_tags, all_symbol_ranges) = (symbol_def_ranges0 
-  dict_Basic_classes_Ord_abifeature dict_Abi_classes_AbiFeatureTagEquiv_abifeature img2) in
+definition defined_symbols  :: " 'abifeature Ord_class \<Rightarrow> 'abifeature AbiFeatureTagEquiv_class \<Rightarrow> 'abifeature annotated_memory_image \<Rightarrow>(symbol_definition)list "  where 
+     " defined_symbols dict_Basic_classes_Ord_abifeature dict_Abi_classes_AbiFeatureTagEquiv_abifeature img3 = ( 
+    (let (all_symbol_tags, all_symbol_ranges) = (symbol_def_ranges 
+  dict_Basic_classes_Ord_abifeature dict_Abi_classes_AbiFeatureTagEquiv_abifeature img3) in
     Lem_list.mapMaybe (\<lambda> tag .  
         (case  tag of
-            SymbolDef0(ent) => Some ent
+            SymbolDef(ent) => Some ent
             | _ => failwith (''impossible: non-symbol def in list of symbol defs'')
         )) all_symbol_tags))"
 
